Outline finiteness

fairis/fairness_finiteness.v
@@ -76,15 +76,16 @@ Section finitary.
   end.
 
   Definition map_underlying_trace {M : FairModel} {LM: LiveModel Λ M} (aux : auxiliary_trace LM) :=
-    (trace_map (λ s, ls_under s) (λ lab, get_role lab) aux).
+    (trace_map (λ s, ls_under $ ls_data s) (λ lab, get_role lab) aux).
 
   Program Definition enumerate_next extr (fmodtr: auxiliary_trace LM) c' oζ:
-    list (LM * @mlabel LM) :=
+    list (LiveStateData Λ M * @mlabel LM) :=
     let δ1 := trace_last fmodtr in
     '(s2, ℓ) ← (δ1.(ls_under), None) :: enum_inner extr (map_underlying_trace fmodtr) c' oζ;
-    d ← enumerate_dom_gsets' (dom δ1.(ls_fuel) ∪ live_roles _ s2);
-    fs ← enum_gmap_bounded' (live_roles _ s2 ∪ d) (max_gmap δ1.(ls_fuel) `max` LM.(lm_fl) s2);
-    ms ← enum_gmap_range_bounded' (live_roles _ s2 ∪ d) (locales_of_list c'.1);
+    d ← enumerate_dom_gsets' (dom (ls_fuel δ1) ∪ live_roles _ s2);
+    (* ms ← enum_gmap_range_bounded' (live_roles _ s2 ∪ d) (locales_of_list c'.1); *)
+    let fss := enumerate_subdomain_gmap d (max_gmap (ls_fuel δ1) `max` LM.(lm_fl) s2) in
+    ms ← enum_gmap_range_bounded' (list_to_set $ locales_of_list c'.1) fss;
     let ℓ' := match ℓ with
               | None => match oζ with
                          Some ζ => Silent_step ζ
@@ -96,17 +97,29 @@ Section finitary.
                          end
               end in
     mret ({| ls_under := s2;
-             ls_fuel := `fs;
-             (* ls_fuel_dom := proj2_sig fs; *) (* TODO: why this does not work?*)
-             ls_mapping := `ms ;
+             ls_map := `ms;
           |}, ℓ').
-  Next Obligation.
-    intros ??????????. destruct fs as [? Heq]. rewrite /= Heq //. set_solver.
-  Qed.
-  Next Obligation.
-    intros ??????????. destruct fs as [? Heq]. destruct ms as [? Heq'].
-    rewrite /= Heq //.
-  Qed.
+
+  Local Instance condition_1_decision x :
+    Decision
+     (∀ (ζ ζ' : locale Λ) (fs fs' : gmap (fmrole M) nat),
+        ζ ≠ ζ' → ls_map x !! ζ = Some fs → ls_map x !! ζ' = Some fs' → fs ##ₘ fs').
+  Proof. apply make_decision. Qed.
+
+  Definition to_ls (x: LiveStateData Λ M) : option LM :=
+    match decide (∀ ζ ζ' fs fs', ζ ≠ ζ' → x.(ls_map) !! ζ = Some fs → x.(ls_map) !! ζ' = Some fs' → fs ##ₘ fs')
+    with
+    | right _ => None
+    | left Hdisj =>
+        match decide (∀ ρ, ρ ∈ M.(live_roles) x.(ls_under) → ∃ ζ fs, x.(ls_map) !! ζ = Some fs ∧ ρ ∈ dom fs) with
+        | right _ => None
+        | left Hlive => Some {| ls_data := x; ls_map_disj := Hdisj; ls_map_live := Hlive |}
+        end
+    end.
+
+  Definition enumerate_next_valid extr (fmodtr: auxiliary_trace LM) c' oζ: list (LM * @mlabel LM) :=
+    let ns := enumerate_next extr fmodtr c' oζ in
+    omap (λ '(x, ℓ), (λ x, (x, ℓ)) <$> to_ls x) ns.
 
   Lemma valid_state_evolution_finitary_fairness (φ: execution_trace Λ -> auxiliary_trace LM -> Prop) :
     rel_finitary (valid_lift_fairness (λ extr auxtr, ξ extr (map_underlying_trace auxtr) ∧ φ extr auxtr)).
@@ -115,9 +128,18 @@ Section finitary.
     intros ex atr [e' σ'] oζ.
     eapply finite_smaller_card_nat.
     simpl.
-    eapply (in_list_finite (enumerate_next ex atr (e',σ') oζ)).
+    eapply (in_list_finite (enumerate_next_valid ex atr (e',σ') oζ)).
     intros [δ' ℓ] [[Hlbl [Htrans Htids]] [Hξ Hφ]].
-    unfold enumerate_next. apply elem_of_list_bind.
+    unfold enumerate_next_valid.
+
+    apply elem_of_list_omap.
+    exists (δ'.(ls_data), ℓ).
+
+    split; last first.
+    { admit. }
+
+    unfold enumerate_next.
+    apply elem_of_list_bind.
     exists (δ'.(ls_under), match ℓ with Take_step l _ => Some l | _ => None end).
     split; last first.
     { destruct ℓ as [ρ tid' | |].
@@ -125,78 +147,79 @@ Section finitary.
         by apply enum_inner_spec.
       - apply elem_of_cons; left. f_equal. inversion Htrans as (?&?&?&?&?); done.
       - apply elem_of_cons; right. inversion Htrans as (?&?). by apply enum_inner_spec. }
-    apply elem_of_list_bind. eexists (dom $ δ'.(ls_fuel)). split; last first.
+    apply elem_of_list_bind. eexists (dom $ ls_fuel δ'). split; last first.
     { apply enumerate_dom_gsets'_spec. destruct ℓ as [ρ tid' | |].
       - inversion Htrans as (?&?&?&?&?&?&?). intros ρ' Hin. destruct (decide (ρ' ∈ live_roles _ δ')); first set_solver.
         destruct (decide (ρ' ∈ dom $ ls_fuel (trace_last atr))); first set_solver. set_solver.
       - inversion Htrans as (?&?&?&?&?). set_solver.
       - inversion Htrans as (?&?&?&?&?). done. }
     apply elem_of_list_bind.
-    assert (Hfueldom: dom δ'.(ls_fuel) = live_roles M δ' ∪ dom (ls_fuel δ')).
+    assert (Hfueldom: dom $ ls_fuel δ' = live_roles M δ' ∪ dom (ls_fuel δ')).
     { rewrite subseteq_union_1_L //. apply ls_fuel_dom. }
-    eexists (δ'.(ls_fuel) ↾ Hfueldom); split; last first.
-    { eapply enum_gmap_bounded'_spec; split =>//.
-      intros ρ f Hsome. destruct ℓ as [ρ' tid' | |].
-      - destruct (decide (ρ = ρ')) as [-> | Hneq].
-        + inversion Htrans as [? Hbig]. destruct Hbig as (Hmap&Hleq&?&Hlim&?&?).
-          destruct (decide (ρ' ∈ live_roles _ δ')).
-          * rewrite Hsome /= in Hlim.
-            assert (Hlive: ρ' ∈ live_roles _ δ') by set_solver.
-            specialize (Hlim Hlive). lia.
-          * unfold fuel_decr in Hleq.
-            apply elem_of_dom_2 in Hmap. rewrite ls_same_doms in Hmap.
-            pose proof Hsome as Hsome'. apply elem_of_dom_2 in Hsome'.
-            specialize (Hleq ρ' ltac:(done) ltac:(done)).
-            assert(must_decrease ρ' (Some ρ') (trace_last atr) δ' (Some tid')) as Hmd; first by constructor 3.
-            specialize (Hleq Hmd). rewrite Hsome /= in Hleq.
-            apply elem_of_dom in Hmap as [? Heq]. rewrite Heq in Hleq.
-            pose proof (max_gmap_spec _ _ _ Heq). simpl in *. lia.
-        + inversion Htrans as [? Hbig]. destruct Hbig as (Hmap&?&Hleq'&?&Hnew&?).
-          destruct (decide (ρ ∈ dom $ ls_fuel (trace_last atr))) as [Hin|Hnotin].
-          * assert (Hok: oleq (ls_fuel δ' !! ρ) (ls_fuel (trace_last atr) !! ρ)).
-            { unfold fuel_must_not_incr in *.
-              assert (ρ ∈ dom $ ls_fuel (trace_last atr)) by SS.
-              specialize (Hleq' ρ ltac:(done) ltac:(congruence)) as [Hleq'|Hleq'] =>//. apply elem_of_dom_2 in Hsome. set_solver. }
-            rewrite Hsome in Hok. destruct (ls_fuel (trace_last atr) !! ρ) as [f'|] eqn:Heqn; last done.
-            pose proof (max_gmap_spec _ _ _ Heqn). simpl in *. lia.
-          * assert (Hok: oleq (ls_fuel δ' !! ρ) (Some (LM.(lm_fl) δ'))).
-            { apply Hnew. apply elem_of_dom_2 in Hsome. set_solver. }
-            rewrite Hsome in Hok. simpl in Hok. lia.
-      - inversion Htrans as [? [? [Hleq [Hincl Heq]]]]. specialize (Hleq ρ).
-        assert (ρ ∈ dom $ ls_fuel (trace_last atr)) as Hin.
-        { apply elem_of_dom_2 in Hsome. set_solver. }
-        specialize (Hleq Hin ltac:(done)) as [Hleq|Hleq].
-        + rewrite Hsome in Hleq. destruct (ls_fuel (trace_last atr) !! ρ) as [f'|] eqn:Heqn.
-          * pose proof (max_gmap_spec _ _ _ Heqn). simpl in *.
-            rewrite Heqn in Hleq.
-            lia.
-          * simpl in *. rewrite Heqn in Hleq. done.
-        + apply elem_of_dom_2 in Hsome. set_solver.
-      - inversion Htrans as [? [? [Hleq [Hnew Hfalse]]]]. done. }
-    apply elem_of_list_bind.
-    assert (Hmappingdom: dom δ'.(ls_mapping) = live_roles M δ' ∪ dom (ls_fuel δ')).
-    { rewrite -Hfueldom ls_same_doms //. }
-    exists (δ'.(ls_mapping) ↾ Hmappingdom); split; last first.
-    { eapply enum_gmap_range_bounded'_spec; split=>//.
-      intros ρ' tid' Hsome. unfold tids_smaller in *.
-      apply locales_of_list_from_locale_from. eauto. }
-    rewrite elem_of_list_singleton; f_equal.
-    - destruct δ'; simpl. f_equal; apply ProofIrrelevance.
-    - destruct ℓ; simpl; destruct oζ =>//; by inversion Hlbl.
-      Unshelve.
-      + intros ??. apply make_decision.
-      + intros. apply make_proof_irrel.
-      + done.
-      + done.
-  Qed.
+  Admitted.
+  (*   eexists (ls_fuel δ' ↾ Hfueldom); split; last first. *)
+  (*   { eapply enum_gmap_bounded'_spec; split =>//. *)
+  (*     intros ρ f Hsome. destruct ℓ as [ρ' tid' | |]. *)
+  (*     - destruct (decide (ρ = ρ')) as [-> | Hneq]. *)
+  (*       + inversion Htrans as [? Hbig]. destruct Hbig as (Hmap&Hleq&?&Hlim&?&?). *)
+  (*         destruct (decide (ρ' ∈ live_roles _ δ')). *)
+  (*         * rewrite Hsome /= in Hlim. *)
+  (*           assert (Hlive: ρ' ∈ live_roles _ δ') by set_solver. *)
+  (*           specialize (Hlim Hlive). lia. *)
+  (*         * unfold fuel_decr in Hleq. *)
+  (*           apply elem_of_dom_2 in Hmap. rewrite ls_same_doms in Hmap. *)
+  (*           pose proof Hsome as Hsome'. apply elem_of_dom_2 in Hsome'. *)
+  (*           specialize (Hleq ρ' ltac:(done) ltac:(done)). *)
+  (*           assert(must_decrease ρ' (Some ρ') (trace_last atr) δ' (Some tid')) as Hmd; first by constructor 3. *)
+  (*           specialize (Hleq Hmd). rewrite Hsome /= in Hleq. *)
+  (*           apply elem_of_dom in Hmap as [? Heq]. rewrite Heq in Hleq. *)
+  (*           pose proof (max_gmap_spec _ _ _ Heq). simpl in *. lia. *)
+  (*       + inversion Htrans as [? Hbig]. destruct Hbig as (Hmap&?&Hleq'&?&Hnew&?). *)
+  (*         destruct (decide (ρ ∈ dom $ ls_fuel (trace_last atr))) as [Hin|Hnotin]. *)
+  (*         * assert (Hok: oleq (ls_fuel δ' !! ρ) (ls_fuel (trace_last atr) !! ρ)). *)
+  (*           { unfold fuel_must_not_incr in *. *)
+  (*             assert (ρ ∈ dom $ ls_fuel (trace_last atr)) by SS. *)
+  (*             specialize (Hleq' ρ ltac:(done) ltac:(congruence)) as [Hleq'|Hleq'] =>//. apply elem_of_dom_2 in Hsome. set_solver. } *)
+  (*           rewrite Hsome in Hok. destruct (ls_fuel (trace_last atr) !! ρ) as [f'|] eqn:Heqn; last done. *)
+  (*           pose proof (max_gmap_spec _ _ _ Heqn). simpl in *. lia. *)
+  (*         * assert (Hok: oleq (ls_fuel δ' !! ρ) (Some (LM.(lm_fl) δ'))). *)
+  (*           { apply Hnew. apply elem_of_dom_2 in Hsome. set_solver. } *)
+  (*           rewrite Hsome in Hok. simpl in Hok. lia. *)
+  (*     - inversion Htrans as [? [? [Hleq [Hincl Heq]]]]. specialize (Hleq ρ). *)
+  (*       assert (ρ ∈ dom $ ls_fuel (trace_last atr)) as Hin. *)
+  (*       { apply elem_of_dom_2 in Hsome. set_solver. } *)
+  (*       specialize (Hleq Hin ltac:(done)) as [Hleq|Hleq]. *)
+  (*       + rewrite Hsome in Hleq. destruct (ls_fuel (trace_last atr) !! ρ) as [f'|] eqn:Heqn. *)
+  (*         * pose proof (max_gmap_spec _ _ _ Heqn). simpl in *. *)
+  (*           rewrite Heqn in Hleq. *)
+  (*           lia. *)
+  (*         * simpl in *. rewrite Heqn in Hleq. done. *)
+  (*       + apply elem_of_dom_2 in Hsome. set_solver. *)
+  (*     - inversion Htrans as [? [? [Hleq [Hnew Hfalse]]]]. done. } *)
+  (*   apply elem_of_list_bind. *)
+  (*   assert (Hmappingdom: dom δ'.(ls_mapping) = live_roles M δ' ∪ dom (ls_fuel δ')). *)
+  (*   { rewrite -Hfueldom ls_same_doms //. } *)
+  (*   exists (δ'.(ls_mapping) ↾ Hmappingdom); split; last first. *)
+  (*   { eapply enum_gmap_range_bounded'_spec; split=>//. *)
+  (*     intros ρ' tid' Hsome. unfold tids_smaller in *. *)
+  (*     apply locales_of_list_from_locale_from. eauto. } *)
+  (*   rewrite elem_of_list_singleton; f_equal. *)
+  (*   - destruct δ'; simpl. f_equal; apply ProofIrrelevance. *)
+  (*   - destruct ℓ; simpl; destruct oζ =>//; by inversion Hlbl. *)
+  (*     Unshelve. *)
+  (*     + intros ??. apply make_decision. *)
+  (*     + intros. apply make_proof_irrel. *)
+  (*     + done. *)
+  (*     + done. *)
+  (* Qed. *)
 End finitary.
 
 Section finitary_simple.
   Context `{M: FairModel}.
   Context `{Λ: language}.
-  Context `{LM: LiveModel Λ M}.
   Context `{EqDecision M}.
-  Context `{EqDecision (locale Λ)}.
+  Context `{Countable (locale Λ)}.
+  Context `{LM: LiveModel Λ M}.
 
   Context `{HPI0: forall s x, ProofIrrel ((let '(s', ℓ) := x in M.(fmtrans) s ℓ s'): Prop) }.
 
@@ -208,136 +231,32 @@ Section finitary_simple.
   Lemma enum_inner_spec_simple (s1 s2: M) ℓ:
     M.(fmtrans) s1 ℓ s2 -> (s2, ℓ) ∈ enum_inner_simple s1.
   Proof.
-    intros H. unfold enum_inner. rewrite elem_of_list_fmap.
-    exists (exist _ (s2, ℓ) H). split =>//. apply elem_of_enum.
+    intros Ht. unfold enum_inner. rewrite elem_of_list_fmap.
+    exists (exist _ (s2, ℓ) Ht). split =>//. apply elem_of_enum.
   Qed.
 
-  Program Definition enumerate_next_simple (δ1: LM) (oζ : olocale Λ) (c': cfg Λ):
-    list (LM * @mlabel LM) :=
-    '(s2, ℓ) ← (δ1.(ls_under), None) :: enum_inner_simple δ1.(ls_under);
-    d ← enumerate_dom_gsets' (dom δ1.(ls_fuel) ∪ live_roles _ s2);
-    fs ← enum_gmap_bounded' (live_roles _ s2 ∪ d) (max_gmap δ1.(ls_fuel) `max` LM.(lm_fl) s2);
-    ms ← enum_gmap_range_bounded' (live_roles _ s2 ∪ d) (locales_of_list c'.1);
-    let ℓ' := match ℓ with
-              | None => match oζ with
-                         Some ζ => Silent_step ζ
-                       | None => Config_step
-                       end
-              | Some ℓ => match oζ with
-                         | None => Config_step
-                         | Some ζ => Take_step ℓ ζ
-                         end
-              end in
-    mret ({| ls_under := s2;
-             ls_fuel := `fs;
-             (* ls_fuel_dom := proj2_sig fs; *) (* TODO: why this does not work?*)
-             ls_mapping := `ms ;
-          |}, ℓ').
-  Next Obligation.
-    intros ??????????. destruct fs as [? Heq]. rewrite /= Heq //. set_solver.
-  Qed.
-  Next Obligation.
-    intros ??????????. destruct fs as [? Heq]. destruct ms as [? Heq'].
-    rewrite /= Heq //.
-  Qed.
-
-  (* TODO: Derive this from the stronger version *)
   Lemma valid_state_evolution_finitary_fairness_simple (φ: execution_trace Λ -> auxiliary_trace LM -> Prop) :
     rel_finitary (valid_lift_fairness φ).
-  Proof.
-    intros extr auxtr [e' σ'] oζ.
-    eapply finite_smaller_card_nat.
-    eapply (in_list_finite (enumerate_next_simple (trace_last auxtr) oζ (e',σ'))).
-    intros [δ2 ℓ] [[Hlab [Htrans Hsmall]] ?].
-    unfold enumerate_next. apply elem_of_list_bind.
-    exists (δ2.(ls_under), match ℓ with Take_step l _ => Some l | _ => None end).
-    split; last first.
-    { destruct ℓ as [ρ tid' | |].
-      - inversion Htrans as [Htrans']. apply elem_of_cons; right. by apply enum_inner_spec_simple.
-      - apply elem_of_cons; left. f_equal. inversion Htrans as (?&?&?&?&?); done.
-      - apply elem_of_cons; right. inversion Htrans as (?&?). by apply enum_inner_spec_simple. }
-    apply elem_of_list_bind. eexists (dom $ δ2.(ls_fuel)). split; last first.
-    { apply enumerate_dom_gsets'_spec. destruct ℓ as [ρ tid' | |].
-      - inversion Htrans as (?&?&?&?&?&?&?). intros ρ' Hin. destruct (decide (ρ' ∈ live_roles _ δ2)); first set_solver.
-        destruct (decide (ρ' ∈ dom $ ls_fuel (trace_last auxtr))); first set_solver. set_solver.
-      - inversion Htrans as (?&?&?&?&?). set_solver.
-      - inversion Htrans as (?&?&?&?&?). done. }
-    apply elem_of_list_bind.
-    assert (Hfueldom: dom δ2.(ls_fuel) = live_roles M δ2 ∪ dom (ls_fuel δ2)).
-    { rewrite subseteq_union_1_L //. apply ls_fuel_dom. }
-
-    eexists (δ2.(ls_fuel) ↾ Hfueldom); split; last first.
-    { eapply enum_gmap_bounded'_spec; split =>//.
-      intros ρ f Hsome. destruct ℓ as [ρ' tid' | |].
-      - destruct (decide (ρ = ρ')) as [-> | Hneq].
-        + inversion Htrans as [? Hbig]. destruct Hbig as (Hmap&Hleq&?&Hlim&?&?).
-          destruct (decide (ρ' ∈ live_roles _ δ2)).
-          * rewrite Hsome /= in Hlim.
-            assert (Hlive: ρ' ∈ live_roles _ δ2) by set_solver.
-            specialize (Hlim Hlive). lia.
-          * unfold fuel_decr in Hleq.
-            apply elem_of_dom_2 in Hmap. rewrite ls_same_doms in Hmap.
-            pose proof Hsome as Hsome'. apply elem_of_dom_2 in Hsome'.
-            specialize (Hleq ρ' ltac:(done) ltac:(done)).
-            assert(must_decrease ρ' (Some ρ') (trace_last auxtr) δ2 (Some tid')) as Hmd; first by constructor 3.
-            specialize (Hleq Hmd). rewrite Hsome /= in Hleq.
-            apply elem_of_dom in Hmap as [? Heq]. rewrite Heq in Hleq.
-            pose proof (max_gmap_spec _ _ _ Heq). simpl in *. lia.
-        + inversion Htrans as [? Hbig]. destruct Hbig as (Hmap&?&Hleq'&?&Hnew&?).
-          destruct (decide (ρ ∈ dom $ ls_fuel (trace_last auxtr))) as [Hin|Hnotin].
-          * assert (Hok: oleq (ls_fuel δ2 !! ρ) (ls_fuel (trace_last auxtr) !! ρ)).
-            { unfold fuel_must_not_incr in *.
-              assert (ρ ∈ dom $ ls_fuel (trace_last auxtr)) by SS.
-              specialize (Hleq' ρ ltac:(done) ltac:(congruence)) as [Hleq'|Hleq'] =>//. apply elem_of_dom_2 in Hsome. set_solver. }
-            rewrite Hsome in Hok. destruct (ls_fuel (trace_last auxtr) !! ρ) as [f'|] eqn:Heqn; last done.
-            pose proof (max_gmap_spec _ _ _ Heqn). simpl in *. lia.
-          * assert (Hok: oleq (ls_fuel δ2 !! ρ) (Some (LM.(lm_fl) δ2))).
-            { apply Hnew. apply elem_of_dom_2 in Hsome. set_solver. }
-            rewrite Hsome in Hok. simpl in Hok. lia.
-      - inversion Htrans as [? [? [Hleq [Hincl Heq]]]]. specialize (Hleq ρ).
-        assert (ρ ∈ dom $ ls_fuel (trace_last auxtr)) as Hin.
-        { apply elem_of_dom_2 in Hsome. set_solver. }
-        specialize (Hleq Hin ltac:(done)) as [Hleq|Hleq].
-        + rewrite Hsome in Hleq. destruct (ls_fuel (trace_last auxtr) !! ρ) as [f'|] eqn:Heqn; last done.
-          pose proof (max_gmap_spec _ _ _ Heqn). simpl in *. lia.
-        + apply elem_of_dom_2 in Hsome. set_solver.
-      - inversion Htrans as [? [? [Hleq [Hnew Hfalse]]]]. done. }
-    apply elem_of_list_bind.
-    assert (Hmappingdom: dom δ2.(ls_mapping) = live_roles M δ2 ∪ dom (ls_fuel δ2)).
-    { rewrite -Hfueldom ls_same_doms //. }
-
-    exists (δ2.(ls_mapping) ↾ Hmappingdom); split; last first.
-    { eapply enum_gmap_range_bounded'_spec; split=>//.
-      intros ρ' tid' Hsome. unfold tids_smaller in *.
-      apply locales_of_list_from_locale_from. eauto. }
-    rewrite elem_of_list_singleton; f_equal.
-    - destruct δ2; simpl. f_equal; apply ProofIrrelevance.
-    - destruct ℓ; simpl; destruct oζ =>//; by inversion Hlab.
-      Unshelve.
-      + intros ??. apply make_decision.
-      + intros. apply make_proof_irrel.
-      + done.
-      + done.
-  Qed.
+  Proof. Admitted.
 End finitary_simple.
 
 (* TODO: Why do we need [LM] explicit here? *)
-Definition live_rel `(LM: LiveModel Λ M) `{Countable (locale Λ)}
+Definition live_rel `{Countable (locale Λ)} `(LM: LiveModel Λ M)
            (ex : execution_trace Λ) (aux : auxiliary_trace LM) :=
   live_tids (LM:=LM) (trace_last ex) (trace_last aux).
 
-Definition sim_rel `(LM: LiveModel Λ M) `{Countable (locale Λ)}
+Definition sim_rel `{Countable (locale Λ)} `(LM: LiveModel Λ M)
            (ex : execution_trace Λ) (aux : auxiliary_trace LM) :=
   valid_state_evolution_fairness ex aux ∧ live_rel LM ex aux.
 
-Definition sim_rel_with_user `(LM: LiveModel Λ M) `{Countable (locale Λ)}
+Definition sim_rel_with_user `{Countable (locale Λ)} `(LM: LiveModel Λ M)
            (ξ : execution_trace Λ -> finite_trace M (option (fmrole M)) -> Prop)
   (ex : execution_trace Λ) (aux : auxiliary_trace LM) :=
   sim_rel LM ex aux ∧ ξ ex (map_underlying_trace aux).
 
 (* TODO: Maybe redefine [sim_rel_with_user] in terms of [valid_lift_fairness] *)
-Lemma valid_lift_fairness_sim_rel_with_user `{LM:LiveModel Λ Mdl}
-      `{Countable (locale Λ)}
+Lemma valid_lift_fairness_sim_rel_with_user
+      `{Countable (locale Λ)} `{LM:LiveModel Λ Mdl}
       (ξ : execution_trace Λ → finite_trace Mdl (option $ fmrole Mdl) →
            Prop) extr atr :
   valid_lift_fairness
@@ -346,8 +265,8 @@ Lemma valid_lift_fairness_sim_rel_with_user `{LM:LiveModel Λ Mdl}
   sim_rel_with_user LM ξ extr atr.
 Proof. split; [by intros [Hvalid [Hlive Hξ]]|by intros [[Hvalid Hlive] Hξ]]. Qed.
 
-Lemma rel_finitary_sim_rel_with_user_ξ `{LM:LiveModel Λ Mdl}
-      `{Countable (locale Λ)} ξ :
+Lemma rel_finitary_sim_rel_with_user_ξ
+      `{Countable (locale Λ)} `{LM:LiveModel Λ Mdl} ξ :
   rel_finitary ξ → rel_finitary (sim_rel_with_user LM ξ).
 Proof.
   intros Hrel.
@@ -359,12 +278,14 @@ Proof.
     - intros ??. apply make_decision. }
   by eapply valid_state_evolution_finitary_fairness.
   Unshelve.
+  - intros ??. apply make_decision.
   - intros ??. apply make_proof_irrel.
 Qed.
 
-Lemma rel_finitary_sim_rel_with_user_sim_rel `{LM:LiveModel Λ Mdl}
+Lemma rel_finitary_sim_rel_with_user_sim_rel
+      `{Countable (locale Λ)} `{LM:LiveModel Λ Mdl}
       `{EqDecision (mstate LM)} `{EqDecision (mlabel LM)}
-      `{Countable (locale Λ)} ξ :
+      ξ :
   rel_finitary (sim_rel LM) → rel_finitary (sim_rel_with_user LM ξ).
 Proof.
   intros Hrel. eapply rel_finitary_impl; [|done]. by intros ex aux [Hsim _].
